new/golang/theory/typing.v
@@ -19,10 +19,14 @@ Section goose_lang.
 
   Infix "=?" := (String.eqb).
 
-  Fixpoint val (d : struct.descriptor) (field_vals: list (string*val)): val :=
-    match d with
-    | [] => (#())
-    | (f,ft)::fs => (default (zero_val ft) (assocl_lookup field_vals f), val fs field_vals)
+  Definition val (t : go_type) (field_vals: list (string*val)): val :=
+    match t with
+    | structT d => (fix val_struct (fs : list (string*go_type)) :=
+                     match fs with
+                     | [] => (#())
+                     | (f,ft)::fs => (default (zero_val ft) (assocl_lookup field_vals f), val_struct fs)%V
+                     end) d
+    | _ => LitV LitPoison
     end.
 End goose_lang.
 End struct.
@@ -99,7 +103,7 @@ Section typing.
   | has_go_type_struct
       (d : struct.descriptor) fvs
       (Hfields : ∀ f t, In (f, t) d → has_go_type (default (zero_val t) (assocl_lookup fvs f)) t)
-    : has_go_type (struct.val d fvs) (structT d)
+    : has_go_type (struct.val (structT d) fvs) (structT d)
   | has_go_type_ptr (l : loc) : has_go_type #l ptrT
   | has_go_type_func f e v : has_go_type (RecV f e v) funcT
   | has_go_type_func_nil : has_go_type nil funcT
@@ -115,8 +119,8 @@ Section typing.
   Lemma zero_val_has_go_type t :
     has_go_type (zero_val t) t.
   Proof.
-    induction t using go_type_ind; rewrite zero_val_unseal; try econstructor;
-    replace (zero_val_def (structT decls)) with (struct.val decls []).
+    induction t using go_type_ind; rewrite zero_val_unseal; try econstructor.
+    replace (zero_val_def (structT decls)) with (struct.val (structT decls) []).
     {
       econstructor. intros. simpl.
       apply Hfields.
@@ -124,7 +128,7 @@ Section typing.
       split; last done. done.
     }
     induction decls.
-    { simpl. replace (#()) with (struct.val [] []) by done. econstructor. }
+    { simpl. replace (#()) with (struct.val (structT []) []) by done. econstructor. }
     destruct a. simpl.
     f_equal.
     { by rewrite zero_val_unseal. }
@@ -167,7 +171,7 @@ Section typing.
     | stringT => #(str "")
     (* | arrayT (len : nat) (elem : go_type) *)
     | sliceT _ => slice.nil
-    | structT decls => struct.val decls []
+    | structT decls => struct.val t []
     | ptrT => nil
     | funcT => nil
     | interfaceT => interface_nil
@@ -182,7 +186,7 @@ Section typing.
     induction t; try done. simpl.
     induction decls; first done.
     destruct a. simpl.
-    by rewrite zero_val_unseal IHdecls.
+    by rewrite IHdecls zero_val_unseal.
   Qed.
 
   Lemma zero_val_eq :
